\input{mitschrift-header}

Let $P_0, \cdots, P_3$ be the control points of curve $p$ and $P_0, Q_1, Q_2, P_3$
the control points of curve $q$.
We have $\|q(t)-p(t)\|$ over-estimates the true distance between the point $p(t)$ and the curve $q$,
since the distance $\dist(q(t), p)$ is defined by $\min_{t'} \|p(t) - q(t')\|$.
Therefore $\max_{t} \|p(t)-q(t)\|$ over-estimates $\max_t \dist(p(t), q)$.
%
\begin{align}
\min_{t'} \|p(t)-q(t')\| &\leq \|p(t)-q(t)\| \\
\RA \dist(p(t), q) &\leq \|p(t)-q(t)\| \\
\RA \max_t \dist(p(t), q) &\leq \max_t \|p(t)-q(t)\|
\end{align}

\section{Calculating $\argmax_t {\|p(t)-q(t)\|_2^2}$}

We calculate $\argmax_t {\|p(t)-q(t)\|_2^2}$:
%
\begin{align}
\|p(t)-q(t)\|_2^2 &= \|(3(1-t)^2 t P_1 + 3 (1-t) t^2 P_2) - (3(1-t)^2 t Q_1 + 3(1-t) t^2 Q_2)\|_2^2 \\
&= \|3(1-t)^2 t (P_1-Q_1) + 3 (1-t) t^2 (P_2 - Q_2)\|_2^2 \\
&= 9 t^2 (1-t)^2 \| (1-t) (P_1-Q_1) + t (P_2 - Q_2)  \|_2^2 \\
&= 9 t^2 (1-t)^2 \l\| \bpm (1-t) (P_{1x} - Q_{1x}) + t(P_{2x} - Q_{2x}) \\ (1-t) (P_{1y} - Q_{1y}) + t(P_{2y} - Q_{2y}) \epm \r\|_2^2
\end{align}
%
For ease of calculation we introduce variable substitutions:
%
\begin{align}
\alpha_{1x} :&= P_{1x} - Q_{1x} \\
\alpha_{2x} :&= P_{2x} - Q_{2x} \\
\alpha_{1y} :&= P_{1y} - Q_{1y} \\
\alpha_{2y} :&= P_{2y} - Q_{2y} \\
\RA \|p(t)-q(t)\|_2^2 &= 9 t^2 (1-t)^2 [ ((1-t)\alpha_{1x} + t \alpha_{2x})^2 + ((1-t)\alpha_{1y} + t \alpha_{2y})^2 ]
\end{align}
%
Let's calculate the first derivative wrt. $t$ and see what we get:
Well, we obviously get a polynomial of degree 3 and we need to find the roots which
is no fun, so lets's do something else: Triangle inequality.

\section{Using the triangle inequality}

We have $\|a+b\| \leq \|a\| + \|b\|$ for any two vectors $a,b$ and any norm $\|\cdot\|$.
Therefore:
%
\begin{align}
\|p(t)-q(t)\| &= \|(3(1-t)^2 t P_1 + 3 (1-t) t^2 P_2) - (3(1-t)^2 t Q_1 + 3(1-t) t^2 Q_2)\| \\
&\leq \|3(1-t)^2 t (P_1-Q_1)\| + \|3 (1-t) t^2 (P_2 - Q_2)\| =: \psi(t) \\
&= 3(1-t)^2 t \underbrace{\|P_1-Q_1\|}_{:=\alpha_1} + 3 (1-t) t^2 \underbrace{\|P_2 - Q_2\|}_{\alpha_2} \\
&= 3(1-t)^2 t \alpha_1 + 3 (1-t) t^2 \alpha_2 \\
\end{align}
%
Now we have a upper bound $\psi(t)$ for each $t \in [0,1]$.
We maximize it wrt. $t$ and obtain an upper bound for $\dist(p,q)$.
%
\begin{align}
0 &= \partial_t [3(1-t)^2 t \alpha_1 + 3 (1-t) t^2 \alpha_2] \\
\LRA 0 &= \partial_t [(1-2t+t^2)t \alpha_1 + (t^2-t^3) \alpha_2] \\
\LRA 0 &= \partial_t [(t-2t^2+t^3) \alpha_1 + (t^2-t^3) \alpha_2] \\
\LRA 0 &= (1 - 4t+3t^2) \alpha_1 + (2t-3t^2) \alpha_2 \\
\LRA 0 &= \alpha_1 + (2\alpha_2 - 4 \alpha_1)t + (3 \alpha_1 - 3 \alpha_2)t^2 \\
\end{align}
%
And that's just implementation stuff, calculate both roots $t_1, t_2$,
the upper bound then is $\max \{\psi(t_1), \psi(t_2)\}$.
$t_1$ and $t_2$ are probably good candidates for the actual time values
maximizing the distance between $p$ and $q$, therefore one could
calculate:
%
\begin{align}
l_1 :&= \min_{t'} \|p(t_1)-q(t')\| \\
l_2 :&= \min_{t'} \|p(t_2)-q(t')\| \\
l_3 :&= \min_{t'} \|p(t')-q(t_1)\| \\
l_4 :&= \min_{t'} \|p(t')-q(t_2)\| \\
\end{align}
%
Then $\max \{l_1, l_2, l_3, l_4\}$ is a lower bound for the maximum distance of $p$ and $q$.

\section{Estimation without finding roots of polynomials}

We want to do something even simpler.
We know now that:
%
\begin{align*}
\dist(p,q) &\leq \max_t [ 3(1-t)^2 t \alpha_1 + 3 (1-t) t^2 \alpha_2 ]
\end{align*}
%
We want to find the maximum value of both summands.
%
\begin{align*}
f_1(t) :&= (1-t)^2 t = (1-2t+t^2)t = t - 2t^2 + t^3 \\
f_1(1) &= f_1(0) = 0 \\
f_1'(t) &= 3t^2 -4t +1 \\
t_{1,2} :&= \frac{4 \pm \sqrt{16-12}}{6} = \frac {4 \pm 2}6 = \{1, 1/3\} \\
f_1(1/3) &= (2/3)^2 \frac 13 = \frac 49 \frac 13 = \frac{4}{27} \\
f_2(t) :&= (1-t)t^2 = f_1(1-t) \\
\RA f_2(2/3) &= \frac 4{27}
\end{align*}
%
Now we can derive a simper, but coarser estimation:
%
\begin{align*}
\dist(p,q) &\leq \max_t  [ 3(1-t)^2 t \alpha_1 + 3 (1-t) t^2 \alpha_2 ] \\
&\leq \max_t 3(1-t)^2 t \alpha_1 + \max_t 3 (1-t) t^2 \alpha_2 \\
&= \frac 49 \alpha_1 + \frac 49 \alpha_2 = \frac 49 (\alpha_1 + \alpha_2) \\
&= \frac 49 (\|P_1-Q_1\| + \|P_2-Q_2\|)
\end{align*}

\section{Estimation using matrix norms}

For a matrix $A$ and vector $b$ we have $\|A b\|_2 \leq \|A\|_2 \|b\|_2$ where $\|A\|_2$ denotes the spectral norm of $A$.

We have:
%
\begin{align*}
\|p(t)-q(t)\|_2 &= \|3(1-t)^2 t (P_1-Q_1) + 3 (1-t) t^2 (P_2 - Q_2)\|_2 \\
&= \l\| \bpm 3(1-t)^2 t & 3(1-t)t^2 \epm \bpm P_1 - Q_1 \\ P_2 - Q_2 \epm \r\|_2 \\
&= 3 \l\| \underbrace{\bpm (1-t)^2 t & (1-t)t^2 \epm}_{=:A} \underbrace{\bpm P_1 - Q_1 \\ P_2 - Q_2 \epm}_{=: b} \r\|_2 \\
&\leq 3 \l\| \bpm (1-t)^2 t & (1-t)t^2 \epm \r\|_2 \l\| \bpm P_1 - Q_1 \\ P_2 - Q_2 \epm \r\|_2 \\
\end{align*}
%
For this special matrix the spectral norm is equal to the Euklidean norm of the row $A$, so we need to maximize:
%
\begin{align*}
f(t) :&= ((1-t)^2t)^2 + ((1-t)t^2)^2 
\end{align*}
%
We used a CAS to find that $f$ has only one local maximum in the interval $[0,1]$ at $t=1/2$
$f(1/2) = 1/32$, so $\|A\|_2 = \sqrt{1/32} = \sqrt{1/2}\sqrt{1/16} = 1/(4\sqrt 2)$.
Therefore:
%
\begin{align*}
\dist(p,q) &\leq \frac{3}{4\sqrt 2} \l\| \underbrace{\bpm P_1 - Q_1 \\ P_2 - Q_2 \epm}_{=b} \r\|_2
\end{align*}
%
Note that $b$ is in this case a $2\times 2$-matrix, so we need a estimation of its spectral norm.
Standard estimations are $\sqrt{\|b\|_\infty \cdot \|b\|_1}$ and $\|b\|_F$.

\end{document}
